\documentclass{article}
\usepackage{amsfonts}
\usepackage{amsmath}
\usepackage{mathtools}
\usepackage[dvipsnames]{xcolor}
\allowdisplaybreaks
\DeclareMathOperator\E{\mathbb{E}}
\DeclareMathOperator\Var{Var}
\newcommand\highlight[1]{{\color{red}#1}}
\newcommand\denominator{\tfrac{1}{n}\sum_{i = 1}^{n}{(x_{i} - \E X )^{2}}}
\usepackage{fancyhdr}
\pagestyle{fancyplain}
\lhead{Psych 205: Statistical Models}
\rhead{Bi-variate Regression Intuitions}
\lfoot{Foushee}
\cfoot{}
\rfoot{\thispage}
\setlength\parindent{0pt}
\setlength\parindent{0pt}
\begin{document}
The below illustrates three cases as a brief demonstration of why the equation for \(\beta\) for bi-variate regression, given and extended in Homework 2, `makes sense.'\\

Suppose first that \(Y\) was exactly equal to \(X\). We'd like to get a slope of \(1\).
\begin{align*}
\beta &= \frac{\tfrac{1}{n}\sum_{i = 1}^{n}{(x_{i} - \E X )\highlight{(y_{i} - \E Y)}}}{\denominator}\\
&= \frac{\tfrac{1}{n}\sum_{i = 1}^{n}{(x_{i} - \E X )\highlight{(x_{i} - \E X )}}}{\denominator}\\
&= \frac{\denominator}{\denominator} = 1
\end{align*}
Suppose now that \(Y\) is a multiple of \(X\): \(Y = \delta X\). We'd like to get a slope of \(\delta\).
\begin{align*}
\beta &= \frac{\tfrac{1}{n}\sum_{i = 1}^{n}{(x_{i} - \E X)\highlight{(y_{i} - \E Y)}}}{\denominator}\\
&= \frac{\tfrac{1}{n}\sum_{i = 1}^{n}{(x_{i} - \E X)\highlight{(\delta x_{i} - \E[\delta X])}}}{\denominator}\\
&= \frac{\tfrac{1}{n}\sum_{i = 1}^{n}{(x_{i} - \E X)\highlight{(\delta x_{i} - \delta\E X)}}}{\denominator}\\
&= \frac{\tfrac{1}{n}\sum_{i = 1}^{n}{\highlight{\delta}(x_{i} - \E X)^{2}}}{\denominator} = \highlight{\delta}
\end{align*}
Finally, suppose that \(Y\) is a linear function of \(X\): \(Y = \gamma + \delta X\). We'd still like to get a slope of \(\delta\).
\begin{align*}
\beta &= \frac{\tfrac{1}{n}\sum_{i = 1}^{n}{(x_{i} - \E X)\highlight{(y_{i} - \E Y)}}}{\denominator}\\
&= \frac{\tfrac{1}{n}\sum_{i = 1}^{n}{(x_{i} - \E X)\highlight{((\gamma + \delta x_{i}) - \E[\gamma + \delta X])}}}{\denominator}\\
&= \frac{\tfrac{1}{n}\sum_{i = 1}^{n}{(x_{i} - \E X)\highlight{((\gamma + \delta x_{i}) - (\gamma + \delta \E X))}}}{\denominator}\\
&= \frac{\tfrac{1}{n}\sum_{i = 1}^{n}{(x_{i} - \E X)\highlight{((\gamma - \gamma) + \delta(x_{i} - \E X))}}}{\denominator}\\
&= \frac{\tfrac{1}{n}\sum_{i = 1}^{n}{\highlight{\delta}(x_{i} - \E X)^{2}}}{\denominator} = \highlight{\delta}
\end{align*}
\end{document}
